Steel: lex order spec

src/lowparse/LowParse.SteelST.VCList.Sorted.fst
@@ -1,5 +1,6 @@
 module LowParse.SteelST.VCList.Sorted
 include LowParse.SteelST.VCList.Iterator
+include LowParse.Spec.Sorted
 
 module AP = LowParse.SteelST.ArrayPtr
 module R = Steel.ST.Reference
@@ -338,85 +339,6 @@ let nlist_sorted
   end else begin
     nlist_sorted_nonempty j f_order n0 va0 a0
   end
-
-(* Lexicographic order *)
-
-let rec lex_compare
-  (#t: Type)
-  (compare: t -> t -> int)
-  (l1 l2: list t)
-: Tot int
-  (decreases l1)
-= match l1, l2 with
-  | [], [] -> 0
-  | [], _ -> -1
-  | a1 :: q1, [] -> 1
-  | a1 :: q1, a2 :: q2 ->
-    let c = compare a1 a2 in
-    if c = 0
-    then lex_compare compare q1 q2
-    else c
-
-let rec lex_compare_equal
-  (#t: Type)
-  (compare: t -> t -> int)
-  (compare_equal: (
-    (x: t) ->
-    (y: t) ->
-    Lemma
-    (compare x y == 0 <==> x == y)
-  ))
-  (l1: list t)
-  (l2: list t)
-: Lemma
-  (ensures (lex_compare compare l1 l2 == 0 <==> l1 == l2))
-  (decreases l1)
-= match l1 with
-  | [] -> ()
-  | a1 :: q1 ->
-    match l2 with
-    | [] -> ()
-    | a2 :: q2 ->
-      compare_equal a1 a2;
-      lex_compare_equal compare compare_equal q1 q2
-
-let rec lex_compare_trans
-  (#t: Type)
-  (compare: t -> t -> int)
-  (compare_equal: (
-    (x: t) ->
-    (y: t) ->
-    Lemma
-    (compare x y == 0 <==> x == y)
-  ))
-  (compare_trans: (
-    (x: t) ->
-    (y: t) ->
-    (z: t) ->
-    Lemma
-    (requires (compare x y < 0 /\ compare y z < 0))
-    (ensures (compare x z < 0))
-  ))
-  (l1: list t)
-  (l2: list t)
-  (l3: list t)
-: Lemma
-  (requires (lex_compare compare l1 l2 < 0 /\ lex_compare compare l2 l3 < 0))
-  (ensures (lex_compare compare l1 l3 < 0))
-  (decreases l1)
-= match l1 with
-  | [] -> ()
-  | a1 :: q1 ->
-    let a2 :: q2 = l2 in
-    let a3 :: q3 = l3 in
-    compare_equal a1 a2;
-    compare_equal a2 a3;
-    compare_equal a1 a3;
-    if compare a1 a2 = 0 && compare a2 a3 = 0
-    then lex_compare_trans compare compare_equal compare_trans q1 q2 q3
-    else if compare a1 a2 < 0 && compare a2 a3 < 0
-    then compare_trans a1 a2 a3
-    else ()
 
 module I16 = FStar.Int16
 
@@ -857,13 +779,6 @@ let nlist_lex_compare
 
 #pop-options
 
-let lex_order
-  (#t: Type)
-  (compare: t -> t -> int)
-  (l1 l2: list t)
-: Tot bool
-= lex_compare compare l1 l2 < 0
-
 inline_for_extraction
 let nlist_lex_order
   (#k: Ghost.erased parser_kind)
@@ -887,15 +802,6 @@ let nlist_lex_order
     (fun res -> res == lex_order compare va0.contents vb0.contents)
 = let comp = nlist_lex_compare j compare f_compare na0 a0 nb0 b0 in
   return (comp `I16.lt` 0s)
-
-let length_first_lex_order
-  (#t: Type)
-  (compare: t -> t -> int)
-  (l1 l2: list t)
-: Tot bool
-= if List.Tot.length l1 = List.Tot.length l2
-  then lex_order compare l1 l2
-  else List.Tot.length l1 < List.Tot.length l2
 
 inline_for_extraction
 let nlist_length_first_lex_order
