src/lowparse/LowParse.Spec.Sorted.fst
@@ -1,0 +1,96 @@
+module LowParse.Spec.Sorted
+
+(* Lexicographic order *)
+
+let rec lex_compare
+  (#t: Type)
+  (compare: t -> t -> int)
+  (l1 l2: list t)
+: Tot int
+  (decreases l1)
+= match l1, l2 with
+  | [], [] -> 0
+  | [], _ -> -1
+  | a1 :: q1, [] -> 1
+  | a1 :: q1, a2 :: q2 ->
+    let c = compare a1 a2 in
+    if c = 0
+    then lex_compare compare q1 q2
+    else c
+
+let rec lex_compare_equal
+  (#t: Type)
+  (compare: t -> t -> int)
+  (compare_equal: (
+    (x: t) ->
+    (y: t) ->
+    Lemma
+    (compare x y == 0 <==> x == y)
+  ))
+  (l1: list t)
+  (l2: list t)
+: Lemma
+  (ensures (lex_compare compare l1 l2 == 0 <==> l1 == l2))
+  (decreases l1)
+= match l1 with
+  | [] -> ()
+  | a1 :: q1 ->
+    match l2 with
+    | [] -> ()
+    | a2 :: q2 ->
+      compare_equal a1 a2;
+      lex_compare_equal compare compare_equal q1 q2
+
+let rec lex_compare_trans
+  (#t: Type)
+  (compare: t -> t -> int)
+  (compare_equal: (
+    (x: t) ->
+    (y: t) ->
+    Lemma
+    (compare x y == 0 <==> x == y)
+  ))
+  (compare_trans: (
+    (x: t) ->
+    (y: t) ->
+    (z: t) ->
+    Lemma
+    (requires (compare x y < 0 /\ compare y z < 0))
+    (ensures (compare x z < 0))
+  ))
+  (l1: list t)
+  (l2: list t)
+  (l3: list t)
+: Lemma
+  (requires (lex_compare compare l1 l2 < 0 /\ lex_compare compare l2 l3 < 0))
+  (ensures (lex_compare compare l1 l3 < 0))
+  (decreases l1)
+= match l1 with
+  | [] -> ()
+  | a1 :: q1 ->
+    let a2 :: q2 = l2 in
+    let a3 :: q3 = l3 in
+    compare_equal a1 a2;
+    compare_equal a2 a3;
+    compare_equal a1 a3;
+    if compare a1 a2 = 0 && compare a2 a3 = 0
+    then lex_compare_trans compare compare_equal compare_trans q1 q2 q3
+    else if compare a1 a2 < 0 && compare a2 a3 < 0
+    then compare_trans a1 a2 a3
+    else ()
+
+let lex_order
+  (#t: Type)
+  (compare: t -> t -> int)
+  (l1 l2: list t)
+: Tot bool
+= lex_compare compare l1 l2 < 0
+
+let length_first_lex_order
+  (#t: Type)
+  (compare: t -> t -> int)
+  (l1 l2: list t)
+: Tot bool
+= if List.Tot.length l1 = List.Tot.length l2
+  then lex_order compare l1 l2
+  else List.Tot.length l1 < List.Tot.length l2
